Bdd/Count.lean
@@ -1,0 +1,314 @@
+import Bdd.Basic
+import Mathlib.Data.Fintype.Vector
+import Mathlib.Data.Fintype.BigOperators
+import Std.Data.HashMap.Lemmas
+
+namespace Count
+
+def Solution (O : OBdd n m) := { I : Vector Bool n // O.evaluate I = true}
+
+private lemma solution_iff_exists (O : OBdd n m) (i : Fin n) : O.evaluate I = true ↔ ∃ b, I[i] = b ∧ O.evaluate I = true := by simp
+private lemma solution_iff_or (O : OBdd n m) (i : Fin n) :
+    (fun I ↦ O.evaluate I = true) = (fun I ↦ (I[i] = false ∧ O.evaluate I = true) ∨ (I[i] = true ∧ O.evaluate I = true)) := by
+  ext I
+  nth_rw 1 [solution_iff_exists O i]
+  simp only [Bool.exists_bool]
+
+private def my_vector_equiv_vector : List.Vector α n ≃ Vector α n where
+  toFun     := fun l ↦ ⟨l.toList.toArray, .trans List.size_toArray   (List.Vector.toList_length _)⟩
+  invFun    := fun v ↦ ⟨v.toList,         .trans Array.length_toList (Vector.size_toArray       _)⟩
+  left_inv  := fun x ↦ (by simp)
+  right_inv := fun x ↦ (by simp)
+
+private instance instVectorFintype [Fintype α] {n : ℕ} : Fintype (Vector α n) := Fintype.ofEquiv (List.Vector α n) my_vector_equiv_vector
+
+@[simp]
+private lemma my_card_vector [Fintype α] (n : Nat) : Fintype.card (Vector α n) = Fintype.card α ^ n :=
+  .trans (Fintype.ofEquiv_card my_vector_equiv_vector) (card_vector n)
+
+instance instFintypeSolution {O : OBdd n m} : Fintype (Solution O) := Subtype.fintype _
+
+abbrev numSolutions (O : OBdd n m) : Nat := Fintype.card (Solution O)
+
+private lemma numSolutions_eq_card_or (O : OBdd n m) (i : Fin n) :
+    numSolutions O = Fintype.card {I : Vector Bool n // (I[i] = false ∧ O.evaluate I = true) ∨ (I[i] = true ∧ O.evaluate I = true)} :=
+  Fintype.card_congr (Equiv.subtypeEquivProp (solution_iff_or ..))
+
+private lemma card_solution_low (O : OBdd n m) (h : O.1.root = .node j):
+    Fintype.card {I : Vector Bool n // I[O.1.heap[j].var] = false ∧ O.evaluate I = true} = Fintype.card {I : Vector Bool n // I[O.1.heap[j].var] = false ∧ (O.low h).evaluate I = true} :=
+  Fintype.card_congr (Equiv.subtypeEquivProp (by
+    ext I
+    simp only [Fin.getElem_fin, and_congr_right_iff, Bool.coe_iff_coe]
+    intro hf
+    rw [OBdd.evaluate_low_eq_evaluate_set_false]
+    simp only [Fin.getElem_fin, Function.comp_apply]
+    congr
+    rw [← hf]
+    simp only [Vector.set_getElem_self]
+  ))
+
+private lemma card_solution_high (O : OBdd n m) (h : O.1.root = .node j):
+    Fintype.card {I : Vector Bool n // I[O.1.heap[j].var] = true ∧ O.evaluate I = true} = Fintype.card {I : Vector Bool n // I[O.1.heap[j].var] = true ∧ (O.high h).evaluate I = true} :=
+  Fintype.card_congr (Equiv.subtypeEquivProp (by
+    ext I
+    simp only [Fin.getElem_fin, and_congr_right_iff, Bool.coe_iff_coe]
+    intro hf
+    rw [OBdd.evaluate_high_eq_evaluate_set_true]
+    simp only [Fin.getElem_fin, Function.comp_apply]
+    congr
+    rw [← hf]
+    simp only [Vector.set_getElem_self]
+  ))
+
+private lemma aux {i : Fin n} {P Q : Vector Bool n → Prop}: Disjoint (fun I ↦ I[i] = false ∧ P I)  (fun I ↦ I[i] = true ∧ Q I) := by
+  intro p hp1 hp2
+  simp only [le_bot_iff]
+  ext I
+  simp only [Pi.bot_apply, «Prop».bot_eq_false, iff_false]
+  intro contra
+  have hI1 := hp1 I contra
+  have hI2 := hp2 I contra
+  simp_all
+
+private lemma aux_low {O : OBdd n m} {h : O.1.root = .node j}: (O.low h).evaluate (I.set (O.1.heap[j.1].var : Fin n) b) = (O.low h).evaluate I := by
+  have : Nary.IndependentOf (O.low h).evaluate O.1.heap[j.1].var := by
+    apply OBdd.independentOf_lt_root (O := (O.low h)) (i := ⟨O.1.heap[j.1].var.1, ?_⟩)
+    have := OBdd.var_lt_low_var (O := O) (h := h)
+    conv at this =>
+      lhs
+      simp [h, Pointer.toVar_node_eq]
+    exact this
+  simp_all
+
+private lemma aux_high {O : OBdd n m} {h : O.1.root = .node j}: (O.high h).evaluate (I.set (O.1.heap[j.1].var) b) = (O.high h).evaluate I := by
+  have : Nary.IndependentOf (O.high h).evaluate O.1.heap[j.1].var := by
+    apply OBdd.independentOf_lt_root (O := (O.high h)) (i := ⟨O.1.heap[j.1].var.1, ?_⟩)
+    have := OBdd.var_lt_high_var (O := O) (h := h)
+    conv at this =>
+      lhs
+      simp [h, Pointer.toVar_node_eq]
+    exact this
+  simp_all
+
+private lemma numSolutions_node {O : OBdd n m} {j : Fin m} (h : O.1.root = .node j) : numSolutions O + numSolutions O = numSolutions (O.low h) + numSolutions (O.high h) := by
+  nth_rw 1 [numSolutions_eq_card_or O O.1.heap[j].var]
+  rw [Fintype.card_subtype_or_disjoint _ _ aux]
+  · rw [card_solution_low O h]
+    rw [card_solution_high O h]
+    nth_rw 1 [numSolutions_eq_card_or O O.1.heap[j].var]
+    rw [Fintype.card_subtype_or_disjoint _ _ aux]
+    · rw [card_solution_low O h]
+      rw [card_solution_high O h]
+      have h1 : Fintype.card { I // I[O.1.heap[j].var] = false ∧ (O.low h).evaluate I = true } = Fintype.card { I // I[O.1.heap[j].var] = true ∧ (O.low h).evaluate I = true } :=
+        Fintype.card_congr
+          { toFun := fun ⟨I, hI⟩ ↦ ⟨I.set O.1.heap[j].var true, by simp only [Fin.getElem_fin, Vector.getElem_set_self, true_and]; simp_all [aux_low]⟩
+            invFun := fun ⟨I, hI⟩ ↦ ⟨I.set O.1.heap[j].var false, by simp only [Fin.getElem_fin, Vector.getElem_set_self, true_and]; simp_all [aux_low]⟩,
+            left_inv := by rintro ⟨I, hI⟩; simp; rw [← hI.1]; simp
+            right_inv := by rintro ⟨I, hI⟩; simp; rw [← hI.1]; simp
+          }
+      have h2 : Fintype.card { I // I[O.1.heap[j].var] = true ∧ (O.high h).evaluate I = true } = Fintype.card { I // I[O.1.heap[j].var] = false ∧ (O.high h).evaluate I = true } :=
+        Fintype.card_congr
+          { toFun := fun ⟨I, hI⟩ ↦ ⟨I.set O.1.heap[j].var false, by simp only [Fin.getElem_fin, Vector.getElem_set_self, true_and]; simp_all [aux_high]⟩
+            invFun := fun ⟨I, hI⟩ ↦ ⟨I.set O.1.heap[j].var true, by simp only [Fin.getElem_fin, Vector.getElem_set_self, true_and]; simp_all [aux_high]⟩,
+            left_inv := by rintro ⟨I, hI⟩; simp; rw [← hI.1]; simp
+            right_inv := by rintro ⟨I, hI⟩; simp; rw [← hI.1]; simp
+          }
+      nth_rw 1 [h1]
+      nth_rw 1 [h2]
+      calc _
+        _ = Fintype.card { I // I[O.1.heap[j].var] = false ∧ (O.low h).evaluate I = true } + Fintype.card { I // I[O.1.heap[j].var] = true ∧ (O.low h).evaluate I = true } +
+            (Fintype.card { I // I[O.1.heap[j].var] = false ∧ (O.high h).evaluate I = true } + Fintype.card { I // I[O.1.heap[j].var] = true ∧ (O.high h).evaluate I = true }) := by omega
+      rw [← Fintype.card_subtype_or_disjoint _ _ aux]
+      rw [← Fintype.card_subtype_or_disjoint _ _ aux]
+      rw [← numSolutions_eq_card_or _ O.1.heap[j].var]
+      rw [← numSolutions_eq_card_or _ O.1.heap[j].var]
+
+private def Invariant (O : OBdd n m) (s : Std.HashMap (Pointer m) Nat) :=
+  ∀ p (hp : p ∈ s),
+    ∃ ho : Bdd.Ordered ⟨O.1.heap, p⟩,
+      s[p]'hp = numSolutions ⟨⟨O.1.heap, p⟩, ho⟩
+
+private def PostCond (O : OBdd n m) (s r : Std.HashMap (Pointer m) Nat) :=
+  (∀ p,
+    (∀ i, s[p]? = some i → r[p]? = some i) ∧
+    (r[p]? = none → s[p]? = none) ∧
+    (s[p]? = none → (∃ i, r[p]? = some i) → Pointer.Reachable O.1.heap O.1.root p))
+
+private lemma postCond_refl : Reflexive (PostCond O) := by
+  intro _ _
+  constructor
+  · simp_all
+  · constructor
+    · simp_all
+    · rintro _ ⟨_, _⟩
+      simp_all
+
+
+private lemma postCond_terminal (hr : s[O.1.root]? = none) (h : O.1.root = Pointer.terminal b) :
+    PostCond O s (s.insert (Pointer.terminal b) i) := by
+  intro p
+  constructor
+  · intro i hi
+    simp only [Std.HashMap.getElem?_insert, beq_iff_eq]
+    split
+    next heq =>
+      subst heq
+      simp_all
+    next => exact hi
+  · constructor
+    · simp_all
+    · intro hp1 ⟨_, hp2⟩
+      simp only [Std.HashMap.getElem?_insert, beq_iff_eq] at hp2
+      split at hp2
+      next heq =>
+        injection hp2 with hpi
+        subst hpi
+        subst heq
+        rw [h]
+        left
+      next => simp_all
+
+private lemma invariant_false (O : OBdd n m) (s : Std.HashMap (Pointer m) Nat ) (inv : Invariant O s) :
+    Invariant O (s.insert (Pointer.terminal false) 0) := by
+  intro p hp
+  simp only [Std.HashMap.mem_insert, beq_iff_eq] at hp
+  cases hp with
+  | inl hp =>
+    subst hp
+    simp [Bdd.Ordered_of_terminal, numSolutions, Solution]
+  | inr hp =>
+    obtain ⟨ha, hb⟩ := inv p hp
+    use ha
+    rw [Std.HashMap.getElem_insert]
+    simp only [beq_iff_eq]
+    split
+    next heq => subst heq; simp [numSolutions, Solution]
+    next => exact hb
+
+private lemma invariant_true (O : OBdd n m) (s : Std.HashMap (Pointer m) Nat ) (inv : Invariant O s) :
+    Invariant O (s.insert (Pointer.terminal true) (2 ^ n)) := by
+  intro p hp
+  simp only [Std.HashMap.mem_insert, beq_iff_eq] at hp
+  cases hp with
+  | inl hp =>
+    subst hp
+    simp [Bdd.Ordered_of_terminal, numSolutions, Solution]
+  | inr hp =>
+    obtain ⟨ha, hb⟩ := inv p hp
+    use ha
+    rw [Std.HashMap.getElem_insert]
+    simp only [beq_iff_eq]
+    split
+    next heq => subst heq; simp [numSolutions, Solution]
+    next => exact hb
+
+private lemma invariant_node (O : OBdd n m) (s : Std.HashMap (Pointer m) Nat ) (inv : Invariant O s) (h : O.1.root = Pointer.node j) :
+    Invariant O (s.insert (Pointer.node j) (((numSolutions (O.low h)) + (numSolutions (O.high h))) / 2)) := by
+  intro p hp
+  simp only [Std.HashMap.mem_insert, beq_iff_eq] at hp
+  cases hp with
+  | inl hp =>
+    subst hp
+    simp_rw [← h]
+    use O.2
+    simp only [Std.HashMap.getElem_insert_self]
+    symm
+    apply Nat.eq_div_of_mul_eq_left
+    · simp only [ne_eq, OfNat.ofNat_ne_zero, not_false_eq_true]
+    · rw [mul_two]
+      exact numSolutions_node h
+  | inr hp =>
+    obtain ⟨ha, hb⟩ := inv p hp
+    use ha
+    rw [Std.HashMap.getElem_insert]
+    simp only [beq_iff_eq]
+    split
+    next heq =>
+      subst heq
+      simp_rw [← h]
+      symm
+      apply Nat.eq_div_of_mul_eq_left
+      · simp only [ne_eq, OfNat.ofNat_ne_zero, not_false_eq_true]
+      · rw [mul_two]
+        exact numSolutions_node h
+    next => exact hb
+
+private def count_helper (O : OBdd n m) (s : Std.HashMap (Pointer m) Nat ) (inv : Invariant O s) :
+    { r : Std.HashMap (Pointer m) Nat //
+      Invariant O r ∧
+      O.1.root ∈ r ∧
+      PostCond O s r
+    } :=
+  match hr : s[O.1.root]? with
+  | some i => ⟨s, inv, by apply Std.HashMap.isSome_getElem?_iff_mem.mp; simp_all only [Option.isSome_some], postCond_refl s⟩
+  | none =>
+    match h : O.1.root with
+    | .terminal false => ⟨s.insert (.terminal false) 0, invariant_false O s inv, by simp only [Std.HashMap.mem_insert, BEq.rfl, true_or], postCond_terminal hr h⟩
+    | .terminal true => ⟨s.insert (.terminal true) (2 ^ n), invariant_true O s inv, by simp only [Std.HashMap.mem_insert, BEq.rfl, true_or], postCond_terminal hr h⟩
+    | .node j =>
+      let ⟨sl, invl, hl1, hl2⟩ := count_helper (O.low h) s inv
+      let ⟨sh, invh, hh1, hh2⟩ := count_helper (O.high h) sl invl
+      have hlh : (O.low h).1.root ∈ sh := by
+        apply Std.HashMap.mem_iff_isSome_getElem?.mp at hl1
+        apply Option.eq_some_of_isSome at hl1
+        have := (hh2 _).1 _ hl1
+        apply Std.HashMap.mem_iff_isSome_getElem?.mpr
+        apply Option.isSome_of_eq_some
+        exact this
+      ⟨ sh.insert (.node j) ((sh[(O.low h).1.root]'hlh + sh[(O.high h).1.root]'hh1) / 2), (by rw [(invh _ hh1).2]; rw [(invh _ hlh).2]; exact invariant_node O sh invh h), by simp only [Std.HashMap.mem_insert, BEq.rfl, true_or], by
+          intro p
+          constructor
+          · intro i hpi
+            simp only [Std.HashMap.getElem?_insert, beq_iff_eq]
+            split
+            next heq =>
+              subst heq
+              simp_all
+            next =>
+              exact (hh2 _).1 _ ((hl2 _).1 _ hpi)
+          · constructor
+            · intro hn
+              simp only [getElem?_eq_none_iff, Std.HashMap.mem_insert, beq_iff_eq, not_or] at hn
+              rcases hn with ⟨hn1, hn2⟩
+              rw [← getElem?_eq_none_iff] at hn2
+              exact (hl2 _).2.1 ((hh2 _).2.1 hn2)
+            · intro hp1 ⟨_, hp2⟩
+              simp only [Std.HashMap.getElem?_insert, beq_iff_eq] at hp2
+              split at hp2
+              next heq =>
+                injection hp2 with hpi
+                subst hpi
+                subst heq
+                rw [h]
+                left
+              next i _ =>
+                cases hm : sl[p]? with
+                | none =>
+                  trans (O.high h).1.root
+                  · right
+                    rfl
+                    simp only [h, OBdd.high, Bdd.high, Fin.getElem_fin]
+                    right
+                    rfl
+                  · exact (hh2 _).2.2 hm ⟨_, hp2⟩
+                | some val =>
+                  trans (O.low h).1.root
+                  · right
+                    rfl
+                    simp only [h, OBdd.low, Bdd.low, Fin.getElem_fin]
+                    left
+                    rfl
+                  · exact (hl2 _).2.2 hp1 ⟨_, hm⟩
+      ⟩
+termination_by O
+
+def count (O : OBdd n m) : Nat :=
+  let ⟨r, _, hin, _⟩ := count_helper O (Std.HashMap.emptyWithCapacity) (by simp [Invariant])
+  r[O.1.root]'hin
+
+lemma count_corrent {O : OBdd n m} : count O = numSolutions O := by
+  simp only [count]
+  split
+  next _ inv hin _ _ => exact (inv _ hin).2
+
+end Count
